compose/Sem.v
@@ -21,7 +21,8 @@ Set Implicit Arguments.
 
 
 
-Definition Ohs := Midx.t -> { oh: Type & oh }.
+(* Definition Ohs := Midx.t -> { oh: Type & oh }. *)
+Definition Ohs := list { oh: Type & oh }.
 
 Module Frame.
 
@@ -43,7 +44,7 @@ Module Ge.
 
   Inductive find_fptr_owner (ge: t) (fptr: val) (ms: ModSem.t): Prop :=
   | find_fptr_owner_intro
-      (MODSEM: List.find (fun ms0 => Midx.eqb ms.(ModSem.midx) ms0.(ModSem.midx)) (fst ge) = Some ms)
+      (MODSEM: In ms (fst ge))
       if_sig
       (INTERNAL: Genv.find_funct ms.(ModSem.skenv) fptr = Some (Internal if_sig)).
 
@@ -85,7 +86,7 @@ Inductive step (ge: Ge.t): state -> trace -> state -> Prop :=
 | step_init
     args frs ms st_init oh ohs
     (MSFIND: ge.(Ge.find_fptr_owner) (Args.get_fptr args) ms)
-    (OH: ohs ms.(ModSem.midx) = (existT id _ oh))
+    (OH: nth_error ohs ms.(ModSem.midx) = Some (existT id _ oh))
     (INIT: ms.(ModSem.initial_frame) oh args st_init):
     step ge (Callstate args frs ohs)
          E0 (State ((Frame.mk ms st_init) :: frs) ohs)
@@ -100,7 +101,7 @@ Inductive step (ge: Ge.t): state -> trace -> state -> Prop :=
     (FINAL: fr0.(Frame.ms).(ModSem.final_frame) fr0.(Frame.st) oh0 retv)
     (AFTER: fr1.(Frame.ms).(ModSem.after_external) fr1.(Frame.st) oh1 retv st0)
     (OHS: ohs1 = Midx.update ohs0 fr0.(Frame.ms).(ModSem.midx) (existT id _ oh0))
-    (OH: ohs1 fr1.(Frame.ms).(ModSem.midx) = (existT id _ oh1)):
+    (OH: nth_error ohs1 fr1.(Frame.ms).(ModSem.midx) = Some (existT id _ oh1)):
     step ge (State (fr0 :: fr1 :: frs) ohs0)
          E0 (State (((Frame.update_st fr1) st0) :: frs) ohs1)
 .
@@ -123,24 +124,20 @@ Section SEMANTICS.
                                       end).
 
   Definition load_system (skenv: SkEnv.t): (ModSem.t * SkEnv.t) :=
-    (System.modsem Midx.ground skenv, (skenv_fill_internals skenv)).
+    (System.modsem (O: Midx.t) skenv, (skenv_fill_internals skenv)).
 
   Definition load_modsems (skenv: SkEnv.t): list ModSem.t :=
-    Midx.map_with_midx (fun midx md => (Mod.modsem md midx skenv)) p.
+    Midx.mapi (fun midx md => (Mod.modsem md midx skenv)) p.
 
   Definition load_genv (init_skenv: SkEnv.t): Ge.t :=
     let (system, skenv) := load_system init_skenv in
     (system :: (load_modsems init_skenv), init_skenv).
 
   Definition load_owned_heaps (ge: Ge.t): Ohs :=
-    fun midx =>
-      match List.find (fun ms => Midx.eqb midx ms.(ModSem.midx)) (fst ge) with
-      | Some ms => existT id _ ms.(ModSem.initial_owned_heap)
-      | _ => (@existT Type (fun _ => _) unit tt)
-      end
+    map (fun ms => existT id _ ms.(ModSem.initial_owned_heap)) (fst ge)
+  .
       (* List.nth midx (map (fun ms => (existT id _ ms.(ModSem.initial_owned_heap))) (fst ge)) *)
       (*                    (@existT Type (fun _ => _) unit tt) *)
-  .
 
   (* Making dummy_module that calls main? => Then what is sk of it? Memory will be different with physical linking *)
   Inductive initial_state (ge: Ge.t): state -> Prop :=
