proof/SimMod.v
@@ -35,10 +35,14 @@ Context `{SM: SimMem.class} {SS: SimSymb.class SM} {SU: Sound.class}.
     ss: SimSymb.t;
   }.
 
-  Definition to_msp (skenv_link_src skenv_link_tgt: SkEnv.t) (sm: SimMem.t) (mp: t)
-             (SMO: SimMemOh.class ((Mod.modsem (mp.(src)) skenv_link_src).(ModSem.owned_heap))
-                                  ((Mod.modsem (mp.(tgt)) skenv_link_tgt).(ModSem.owned_heap))): ModSemPair.t :=
-    ModSemPair.mk (Mod.modsem (mp.(src)) skenv_link_src) (Mod.modsem (mp.(tgt)) skenv_link_tgt) mp.(ss) sm.
+  Definition to_msp (midx: Midx.t)
+             (skenv_link_src skenv_link_tgt: SkEnv.t) (sm: SimMem.t) (mp: t)
+             (SMO: SimMemOh.class
+                     ((Mod.modsem (mp.(src)) midx skenv_link_src).(ModSem.owned_heap))
+                     ((Mod.modsem (mp.(tgt)) midx skenv_link_tgt).(ModSem.owned_heap)))
+    : ModSemPair.t
+    := ModSemPair.mk (Mod.modsem (mp.(src)) midx skenv_link_src)
+                     (Mod.modsem (mp.(tgt)) midx skenv_link_tgt) mp.(ss) sm.
 
   (* TODO: Actually, ModPair can have idx/ord and transfer it to ModSemPair. *)
   (* Advantage: We can unify ord at Mod state. *)
@@ -47,14 +51,16 @@ Context `{SM: SimMem.class} {SS: SimSymb.class SM} {SU: Sound.class}.
       (SIMSK: SimSymb.wf mp.(ss))
       (SKSRC: mp.(ss).(SimSymb.src) = (Mod.sk mp.(src)))
       (SKTGT: mp.(ss).(SimSymb.tgt) = (Mod.sk mp.(tgt)))
-      (SIMMS: forall skenv_link_src skenv_link_tgt ss_link sm_init_link
+      (SIMMS: forall midx skenv_link_src skenv_link_tgt ss_link sm_init_link
           (INCLSRC: SkEnv.includes skenv_link_src (Mod.sk mp.(src)))
           (INCLTGT: SkEnv.includes skenv_link_tgt (Mod.sk mp.(tgt)))
           (WFSRC: SkEnv.wf skenv_link_src)
           (WFTGT: SkEnv.wf skenv_link_tgt)
           (SSLE: SimSymb.le mp.(ss) ss_link)
           (SIMSKENVLINK: SimSymb.sim_skenv sm_init_link ss_link skenv_link_src skenv_link_tgt),
-          exists SMO, <<SIMMSP: ModSemPair.sim (to_msp skenv_link_src skenv_link_tgt sm_init_link mp SMO)>>).
+          exists SMO, <<SIMMSP: ModSemPair.sim
+                                  (to_msp midx skenv_link_src skenv_link_tgt
+                                          sm_init_link mp SMO)>>).
   (* TODO: quantifying "exists SMO" here looks somewhat dirty... *)
   (* I would like to quantify it directly inside "sim_intro", but I need to put it here because *)
   (* I need to know "owned_heap" type which needs to know "skenv_link_src,tgt". *)
